Common/Maps.v
@@ -8,6 +8,11 @@ Module NMap := FMapAVL.Make backNat_as_OT.
 Module NMapExtra := WProperties_fun Nat_as_OT NMap.
 Module NMapFacts := NMapExtra.F.
 
+Module backZ_as_OT := Backport_OT Z_as_OT.
+Module ZMap := FMapAVL.Make backZ_as_OT.
+Module ZMapExtra := WProperties_fun Z_as_OT ZMap.
+Module ZMapFacts := ZMapExtra.F.
+
 Module N_as_OT := Backport_OT N_as_OT.
 Module BinNatMap := FMapAVL.Make(N_as_OT).
 Module BinNatMapExtra := WProperties_fun N_as_OT BinNatMap.
